validator

tests/pulse/ArithParse.Spec.fst
@@ -13,22 +13,42 @@ type expr =
 | Minus of (expr & expr) // header 254
 | Value of U64.t // header 255
 
-let header_rhs (lhs: U8.t) = if lhs = 255uy then U64.t else unit
+let unit_as_uint64 = (x: U64.t { x == 0uL })
+inline_for_extraction noextract [@@noextract_to "krml"]
+let u_as_uint64 : unit_as_uint64 = 0uL
+
+let header_rhs (lhs: U8.t) = if lhs = 255uy then U64.t else unit_as_uint64
 
 let header = dtuple2 U8.t header_rhs
 
 let parse_header_rhs_kind : parser_kind =
   strong_parser_kind 0 8 None
 
-let parse_header_rhs (lhs: U8.t) : Tot (tot_parser parse_header_rhs_kind (header_rhs lhs)) =
+let parse_header_rhs (lhs: U8.t) : Tot (parser parse_header_rhs_kind (header_rhs lhs)) =
+      if lhs = 255uy
+      then weaken parse_header_rhs_kind parse_u64
+      else weaken parse_header_rhs_kind (parse_ret u_as_uint64)
+
+let tot_parse_header_rhs (lhs: U8.t) : Tot (tot_parser parse_header_rhs_kind (header_rhs lhs)) =
       if lhs = 255uy
       then tot_weaken parse_header_rhs_kind tot_parse_u64
-      else tot_weaken parse_header_rhs_kind tot_parse_empty
+      else tot_weaken parse_header_rhs_kind (tot_parse_ret u_as_uint64)
 
-let parse_header : tot_parser _ header =
-  tot_parse_dtuple2 tot_parse_u8 parse_header_rhs    
+let tot_parse_header : tot_parser _ header =
+  tot_parse_dtuple2 tot_parse_u8 tot_parse_header_rhs    
 
 let parse_header_kind = and_then_kind parse_u8_kind parse_header_rhs_kind
+
+let parse_header : parser parse_header_kind header =
+  parse_dtuple2 parse_u8 parse_header_rhs    
+
+let parse_header_eq () : Lemma (forall x . parse parse_header x == parse tot_parse_header x) =
+  let prf (x: bytes) : Lemma
+    (parse parse_header x == parse tot_parse_header x)
+  = parse_dtuple2_eq parse_u8 parse_header_rhs x;
+    ()
+  in
+  Classical.forall_intro prf
 
 let count_payload (h: header) : Tot nat =
   match h with
@@ -54,29 +74,37 @@ let parse_expr_param : parse_recursive_param = {
   t = expr;
   header = header;
   parse_header_kind = parse_header_kind;
-  parse_header = parse_header;
+  parse_header = tot_parse_header;
   count = count_payload;
   synth_ = synth_expr;
   synth_inj = synth_expr_injective ();
 }
 
-let parse_expr = parse_recursive parse_expr_param
+let tot_parse_expr = parse_recursive parse_expr_param
 
-let serialize_header_rhs (lhs: U8.t) : tot_serializer (parse_header_rhs lhs) =
+let tot_serialize_header_rhs (lhs: U8.t) : tot_serializer (tot_parse_header_rhs lhs) =
   if lhs = 255uy
   then tot_serialize_weaken parse_header_rhs_kind tot_serialize_u64
-  else tot_serialize_weaken parse_header_rhs_kind tot_serialize_empty
+  else tot_serialize_weaken parse_header_rhs_kind (tot_serialize_ret u_as_uint64 (fun _ -> ()))
 
-let serialize_header : tot_serializer parse_header =
-  tot_serialize_dtuple2 tot_serialize_u8 serialize_header_rhs
+let tot_serialize_header : tot_serializer tot_parse_header =
+  tot_serialize_dtuple2 tot_serialize_u8 tot_serialize_header_rhs
+
+let serialize_header_rhs (lhs: U8.t) : serializer (parse_header_rhs lhs) =
+  if lhs = 255uy
+  then serialize_weaken parse_header_rhs_kind serialize_u64
+  else serialize_weaken parse_header_rhs_kind (serialize_ret u_as_uint64 (fun _ -> ()))
+
+let serialize_header : serializer parse_header =
+  serialize_dtuple2 serialize_u8 serialize_header_rhs
 
 let synth_expr_recip
   (x: expr)
 : Tot (parse_recursive_alt_t expr header count_payload)
 = match x with
   | Value v -> (| (| 255uy, v |), [] |)
-  | Minus (v1, v2) -> (| (| 254uy, () |), [v1; v2] |)
-  | Plus p -> (| (| U8.uint_to_t (List.Tot.length p), () |), p |)
+  | Minus (v1, v2) -> (| (| 254uy, u_as_uint64 |), [v1; v2] |)
+  | Plus p -> (| (| U8.uint_to_t (List.Tot.length p), u_as_uint64 |), p |)
 
 let synth_expr_inverse () : Lemma (synth_inverse synth_expr synth_expr_recip) = ()
 
@@ -113,11 +141,11 @@ let level_correct (x: expr) (n: nat) : Lemma
   | _ -> ()
 
 let serialize_expr_param : serialize_recursive_param parse_expr_param = {
-  serialize_header = serialize_header;
+  serialize_header = tot_serialize_header;
   synth_recip = synth_expr_recip;
   synth_inv = synth_expr_inverse ();
   level = level;
   level_correct = level_correct
 }
 
-let serialize_expr : tot_serializer parse_expr = serialize_recursive serialize_expr_param
+let tot_serialize_expr : tot_serializer tot_parse_expr = serialize_recursive serialize_expr_param
