tests/pulse/ArithParse.Impl.fst
@@ -3,6 +3,8 @@ module ArithParse.Impl
 include ArithParse.Spec
 open LowParse.Spec.Base
 open LowParse.Pulse.Base
+open LowParse.Pulse.Combinators
+open LowParse.Pulse.Int
 open LowParse.Pulse.VCList
 open LowParse.Pulse.Recursive
 open Pulse.Lib.Pervasives
@@ -11,6 +13,104 @@ module S = Pulse.Lib.Slice
 module U64 = FStar.UInt64
 module U8 = FStar.UInt8
 module PM = Pulse.Lib.SeqMatch
+
+(* Validation *)
+
+inline_for_extraction noextract [@@noextract_to "krml"]
+let validate_header_rhs (lhs: U8.t) : validator (parse_header_rhs lhs) =
+  ifthenelse_validator
+    (parse_header_rhs lhs)
+    (lhs = 255uy)
+    (fun _ -> validate_weaken parse_header_rhs_kind (validate_u64))
+    (fun _ -> validate_weaken parse_header_rhs_kind (validate_ret u_as_uint64))
+
+inline_for_extraction noextract [@@noextract_to "krml"]
+let validate_header : validator parse_header =
+  validate_dtuple2 validate_u8 (leaf_reader_of_reader read_u8) validate_header_rhs
+
+inline_for_extraction noextract [@@noextract_to "krml"]
+let jump_header_rhs (lhs: U8.t) : jumper (parse_header_rhs lhs) =
+  ifthenelse_jumper
+    (parse_header_rhs lhs)
+    (lhs = 255uy)
+    (fun _ -> jump_ext (jump_u64) (parse_header_rhs lhs))
+    (fun _ -> jump_ext (jump_ret u_as_uint64) (parse_header_rhs lhs))
+
+inline_for_extraction noextract [@@noextract_to "krml"]
+let jump_header : jumper parse_header =
+  jump_dtuple2 jump_u8 (leaf_reader_of_reader read_u8) jump_header_rhs
+
+inline_for_extraction noextract [@@noextract_to "krml"]
+let read_header_rhs (lhs: U8.t) : reader (serialize_header_rhs lhs) =
+  ifthenelse_reader
+    (serialize_header_rhs lhs)
+    (lhs = 255uy)
+    (fun _ -> reader_ext (read_u64) (serialize_header_rhs lhs))
+    (fun _ -> reader_ext (read_ret u_as_uint64 (fun _ -> ())) (serialize_header_rhs lhs))
+
+let read_header () : leaf_reader #_ #_ #_ (serializer_of_tot_serializer tot_serialize_header) =
+  [@@inline_let] let _ = parse_header_eq () in
+  leaf_reader_of_reader
+    (reader_ext (read_dtuple2 jump_u8 read_u8 read_header_rhs) _)
+
+module SZ = FStar.SizeT
+
+#push-options "--ifuel 4"
+
+inline_for_extraction noextract [@@noextract_to "krml"]
+fn impl_validate_count_payload () : validate_recursive_step_count #_ serialize_expr_param =
+  (#va: _)
+  (#pm: _)
+  (a: _)
+  (bound: _)
+  (#rem: _)
+  (prem: _)
+{
+  let h = read_header () a;
+  let Mkdtuple2 kd len = h;
+  if (kd = 255uy) {
+    prem := 0sz;
+    false
+  }
+  else if (kd = 254uy) {
+    prem := 2sz;
+    false
+  } else {
+    let len16 = FStar.Int.Cast.uint8_to_uint16 kd;
+    prem := SZ.uint16_to_sizet len16;
+    false
+  }
+}
+
+let validate_expr : validator tot_parse_expr =
+  [@@inline_let] let _ = parse_header_eq () in
+  validate_recursive serialize_expr_param validate_header (impl_validate_count_payload ())
+
+inline_for_extraction noextract [@@noextract_to "krml"]
+fn impl_jump_count_payload () : jump_recursive_step_count #_ serialize_expr_param =
+  (#va: _)
+  (#pm: _)
+  (a: _)
+  (bound: _)
+{
+  let h = read_header () a;
+  let Mkdtuple2 kd len = h;
+  if (kd = 255uy) {
+    0sz;
+  }
+  else if (kd = 254uy) {
+    2sz;
+  } else {
+    let len16 = FStar.Int.Cast.uint8_to_uint16 kd;
+    SZ.uint16_to_sizet len16;
+  }
+}
+
+let jump_expr : jumper tot_parse_expr =
+  [@@inline_let] let _ = parse_header_eq () in
+  jump_recursive serialize_expr_param jump_header (impl_jump_count_payload ())
+
+(* Low-level data structure *)
 
 noeq
 type expr_t =
@@ -113,7 +213,7 @@ let rec rel
 : Tot slprop
   (decreases high)
 = match low, high with
-  | EUnparsed s, _ -> pts_to_serialized_with_perm (serializer_of_tot_serializer serialize_expr) s high
+  | EUnparsed s, _ -> pts_to_serialized_with_perm (serializer_of_tot_serializer tot_serialize_expr) s high
   | EPlus s, Plus l -> nlist_match_slice_wf (List.Tot.length l) s l rel
   | EMinus pl, Minus ph -> vmatch_pair (vmatch_ref_wf (Minus ph) rel) (vmatch_ref_wf (Minus ph) rel) pl ph
   | EValue vl, Value vh -> eq_as_slprop U64.t vl vh
@@ -128,7 +228,7 @@ let rel'
   | EPlus s, Plus l -> nlist_match_slice0 rel (List.Tot.length l) s l
   | EMinus pl, Minus ph -> vmatch_pair (vmatch_ref rel) (vmatch_ref rel) pl ph
   | EValue vl, Value vh -> eq_as_slprop U64.t vl vh
-  | EUnparsed s, _ -> pts_to_serialized_with_perm (serializer_of_tot_serializer serialize_expr) s high
+  | EUnparsed s, _ -> pts_to_serialized_with_perm (serializer_of_tot_serializer tot_serialize_expr) s high
   | _ -> pure False
 
 let rel_eq
